Reach ber_check_tags call

src/Primitive/Boolean/VstDec.v
@@ -21,66 +21,67 @@ Definition bool_ber_decode_spec : ident * funspec :=
     WITH ctx_p : val, ctx : val, td_p : val, td : TYPE_descriptor,
          bv_pp : val, buf_p : val, buf : list byte,
          res_p : val, size : Z, tag_mode : Z, bv_p : val 
-   PRE[tptr asn_dec_rval_s, tptr asn_codec_ctx_s, tptr type_descriptor_s,
-         tptr (tptr tvoid), tptr tvoid, tuint, tint] 
-    PROP(is_pointer_or_null bv_p; decoder_type td = BOOLEAN_t)
-    PARAMS(res_p; ctx_p; td_p; bv_pp; buf_p; Vint (Int.repr size);
-             Vint (Int.repr tag_mode))
-    GLOBALS()
-    SEP(valid_pointer bv_p;
-        data_at Tsh asn_codec_ctx_s ctx ctx_p;
-        data_at_ Tsh type_descriptor_s td_p;
-        data_at Tsh (tarray tschar (Zlength buf)) (map Vbyte buf) buf_p;
-        data_at Tsh (tptr tvoid) bv_p bv_pp;
-        data_at_ Tsh asn_dec_rval_s res_p)
+    PRE [tptr asn_dec_rval_s, tptr asn_codec_ctx_s, tptr type_descriptor_s,
+          tptr (tptr tvoid), tptr tvoid, tuint, tint] 
+      PROP (is_pointer_or_null bv_p; decoder_type td = BOOLEAN_t)
+      PARAMS (res_p; ctx_p; td_p; bv_pp; buf_p; Vint (Int.repr size);
+                Vint (Int.repr tag_mode))
+      GLOBALS ()
+      SEP (valid_pointer bv_p;
+           data_at Tsh asn_codec_ctx_s ctx ctx_p;
+           data_at_ Tsh type_descriptor_s td_p;
+           data_at Tsh (tarray tschar (Zlength buf)) (map Vbyte buf) buf_p;
+           data_at Tsh (tptr tvoid) bv_p bv_pp;
+           data_at_ Tsh asn_dec_rval_s res_p)
     POST [tvoid]
-      PROP()
-      LOCAL()
-      SEP((* Unchanged by the execution : *)
-          valid_pointer bv_p;
-          data_at Tsh asn_codec_ctx_s ctx ctx_p;
-          data_at_ Tsh type_descriptor_s td_p;
-          data_at Tsh (tarray tschar (Zlength buf)) (map Vbyte buf) buf_p;
-          data_at Tsh (tptr tvoid) bv_p bv_pp;
-          (* Changes according to the exec spec *)
-          let RC_FAIL := 
-              data_at Tsh asn_dec_rval_s (construct_dec_rval 2 0) res_p in
-          if Val.eq bv_p Vnullptr 
-          then RC_FAIL 
-          else match bool_decoder td buf with
-               | Some (r, c) => 
-                 data_at Tsh asn_dec_rval_s (construct_dec_rval 0 c) res_p *
-                 data_at Tsh tuchar (Val.of_bool r) bv_p 
-               | None => RC_FAIL                          
-               end).
+      PROP ()
+      LOCAL ()
+      SEP ((* Unchanged by the execution : *)
+           valid_pointer bv_p;
+           data_at Tsh asn_codec_ctx_s ctx ctx_p;
+           data_at_ Tsh type_descriptor_s td_p;
+           data_at Tsh (tarray tschar (Zlength buf)) (map Vbyte buf) buf_p;
+           data_at Tsh (tptr tvoid) bv_p bv_pp;
+           (* Changes according to the exec spec *)
+           let RC_FAIL := 
+               data_at Tsh asn_dec_rval_s (construct_dec_rval 2 0) res_p in
+           if Val.eq bv_p Vnullptr 
+           then RC_FAIL 
+           else match bool_decoder td buf with
+                | Some (r, c) => 
+                  data_at Tsh asn_dec_rval_s (construct_dec_rval 0 c) res_p *
+                  data_at Tsh tuchar (Val.of_bool r) bv_p 
+                | None => RC_FAIL                          
+                end).
 
 Definition if_post1 bv_p v__res__1 v_tmp_error v_length v_rval 
            res_p ctx ctx_p td_p bv_pp buf buf_p size tag_mode := 
   EX is_inner : bool, EX p : val * type * list byte,
-  PROP()
-  LOCAL(temp _st (if is_inner then fst (fst p) else bv_p); temp _t'11 bv_p;
-  lvar __res__1 (Tstruct _asn_dec_rval_s noattr) v__res__1;
-  lvar _tmp_error (Tstruct _asn_dec_rval_s noattr) v_tmp_error;
-  lvar _length tint v_length;
-  lvar _rval (Tstruct _asn_dec_rval_s noattr) v_rval;
-  temp __res res_p; temp _opt_codec_ctx ctx_p;
-  temp _td td_p; temp _bool_value bv_pp;
-  temp _buf_ptr buf_p;
-  temp _size (Vint (Int.repr size));
-  temp _tag_mode (Vint (Int.repr tag_mode)))
+  PROP ()
+  LOCAL (temp _st (if is_inner then fst (fst p) else bv_p); temp _t'11 bv_p;
+         lvar __res__1 (Tstruct _asn_dec_rval_s noattr) v__res__1;
+         lvar _tmp_error (Tstruct _asn_dec_rval_s noattr) v_tmp_error;
+         lvar _length tint v_length; temp __res res_p; temp _opt_codec_ctx ctx_p;
+         lvar _rval (Tstruct _asn_dec_rval_s noattr) v_rval;
+         temp _td td_p; temp _bool_value bv_pp;
+         temp _buf_ptr buf_p; temp _size (Vint (Int.repr size));
+         temp _tag_mode (Vint (Int.repr tag_mode)))
   SEP (if eq_dec (fst (fst p)) nullval 
        then emp 
        else malloc_token Ews (snd (fst p)) (fst (fst p)) * 
             data_at Ews (tarray tschar 1) (map Vbyte (snd p)) (fst (fst p));
-  data_at_ Tsh (Tstruct _asn_dec_rval_s noattr) v__res__1;
-  data_at_ Tsh (Tstruct _asn_dec_rval_s noattr) v_tmp_error;
-  data_at_ Tsh tint v_length; 
-  data_at_ Tsh (Tstruct _asn_dec_rval_s noattr) v_rval; valid_pointer bv_p;
-  data_at Tsh asn_codec_ctx_s ctx ctx_p;
-  data_at_ Tsh type_descriptor_s td_p;
-  data_at Tsh (tarray tschar (Zlength buf)) (map Vbyte buf) buf_p;
-  data_at Tsh (tptr tvoid) (if is_inner then fst (fst p) else bv_p) bv_pp;
-  data_at_ Tsh asn_dec_rval_s res_p).
+       data_at_ Tsh (Tstruct _asn_dec_rval_s noattr) v__res__1;
+       data_at_ Tsh (Tstruct _asn_dec_rval_s noattr) v_tmp_error;
+       data_at_ Tsh tint v_length; 
+       data_at_ Tsh (Tstruct _asn_dec_rval_s noattr) v_rval; valid_pointer bv_p;
+       data_at Tsh asn_codec_ctx_s ctx ctx_p;
+       data_at_ Tsh type_descriptor_s td_p;
+       data_at Tsh (tarray tschar (Zlength buf)) (map Vbyte buf) buf_p;
+       data_at Tsh (tptr tvoid) (if is_inner then fst (fst p) else bv_p) bv_pp;
+       data_at_ Tsh asn_dec_rval_s res_p).
+
+(*Definition loop_inv1 :=.
+Definition loop_post1 :=.*)
 
 Definition Gprog := ltac:(with_library prog [(_calloc, calloc_spec);
                                               ber_check_tags_spec; 
@@ -101,32 +102,92 @@ Proof.
     forward.
     forward.
     forward_if.
-    destruct eq_dec eqn:ED; unfold fst in *; break_let.
-    - cbn in e; subst.
+    if_tac; break_let.
+    - cbn in H1; subst.
       entailer!.
     - eapply denote_tc_test_eq_split; entailer!.
     - unfold fst in *; rewrite H4.
-      destruct eq_dec; [|congruence].
+      rewrite if_true by reflexivity.
       repeat forward.
+      rewrite if_true by reflexivity.
       entailer!.
-      repeat break_if; entailer!.
     - forward.
       unfold if_post1.
-      destruct eq_dec; [unfold fst in e, H4; congruence|].
-      Exists true.
-      Exists p.
-      destruct eq_dec; [congruence|].
+      rewrite if_false by assumption.
+      Exists true p.
+      rewrite if_false by assumption.
       entailer!.
   * (* _st <> NULL *)
     forward.
     unfold if_post1.
     (* p belongs to inner if, since we didn't reach it, it's uninitialized *)
-    Exists false.
-    Exists (nullval, tptr tvoid, buf).
-    unfold fst; destruct eq_dec; [|congruence].
+    Exists false (nullval, tptr tvoid, buf).
+    rewrite if_true by reflexivity.
     entailer!.
   * (* after the if *)
-    admit.
+    unfold if_post1.
+    Intros is_inner p.
+    forward_loop 
+      (PROP ()
+       LOCAL (temp _st (if is_inner then fst (fst p) else bv_p);
+              lvar __res__1 (Tstruct _asn_dec_rval_s noattr) v__res__1;
+              lvar _tmp_error (Tstruct _asn_dec_rval_s noattr)
+                v_tmp_error; lvar _length tint v_length;
+              temp __res res_p; temp _opt_codec_ctx ctx_p;
+              lvar _rval (Tstruct _asn_dec_rval_s noattr) v_rval;
+              temp _td td_p; temp _bool_value bv_pp;
+              temp _buf_ptr buf_p; temp _size (Vint (Int.repr size));
+              temp _tag_mode (Vint (Int.repr tag_mode)))
+       SEP (if eq_dec (fst (fst p)) nullval
+            then emp
+            else malloc_token Ews (snd (fst p)) (fst (fst p)) * 
+                 data_at Ews (tarray tschar 1) (map Vbyte (snd p)) 
+                         (fst (fst p));
+            data_at_ Tsh (Tstruct _asn_dec_rval_s noattr) v__res__1;
+            data_at_ Tsh (Tstruct _asn_dec_rval_s noattr) v_tmp_error;
+            data_at_ Tsh tint v_length;
+            data_at_ Tsh (Tstruct _asn_dec_rval_s noattr) v_rval;
+            valid_pointer bv_p; data_at Tsh asn_codec_ctx_s ctx ctx_p;
+            data_at_ Tsh type_descriptor_s td_p;
+            data_at Tsh (tarray tschar (Zlength buf)) 
+              (map Vbyte buf) buf_p;
+            data_at Tsh (tptr tvoid)
+              (if is_inner then fst (fst p) else bv_p) bv_pp;
+            data_at_ Tsh asn_dec_rval_s res_p)) 
+      break: 
+      (PROP ()
+       LOCAL (temp _st (if is_inner then fst (fst p) else bv_p);
+              lvar __res__1 (Tstruct _asn_dec_rval_s noattr) v__res__1;
+              lvar _tmp_error (Tstruct _asn_dec_rval_s noattr)
+                v_tmp_error; lvar _length tint v_length;
+              temp __res res_p; temp _opt_codec_ctx ctx_p;
+              lvar _rval (Tstruct _asn_dec_rval_s noattr) v_rval;
+              temp _td td_p; temp _bool_value bv_pp;
+              temp _buf_ptr buf_p; temp _size (Vint (Int.repr size));
+              temp _tag_mode (Vint (Int.repr tag_mode)))
+       SEP (if eq_dec (fst (fst p)) nullval
+            then emp
+            else malloc_token Ews (snd (fst p)) (fst (fst p)) * 
+                 data_at Ews (tarray tschar 1) (map Vbyte (snd p)) 
+                         (fst (fst p));
+            data_at_ Tsh (Tstruct _asn_dec_rval_s noattr) v__res__1;
+            data_at_ Tsh (Tstruct _asn_dec_rval_s noattr) v_tmp_error;
+            data_at_ Tsh tint v_length;
+            data_at_ Tsh (Tstruct _asn_dec_rval_s noattr) v_rval;
+            valid_pointer bv_p; data_at Tsh asn_codec_ctx_s ctx ctx_p;
+            data_at_ Tsh type_descriptor_s td_p;
+            data_at Tsh (tarray tschar (Zlength buf)) 
+              (map Vbyte buf) buf_p;
+            data_at Tsh (tptr tvoid)
+              (if is_inner then fst (fst p) else bv_p) bv_pp;
+            data_at_ Tsh asn_dec_rval_s res_p)).
+    - (* pre-condition = invariant *)
+      entailer!.
+    - (* invariant step to post condition *)
+      forward.
+      entailer!.
+    - (* after the loop *)
+      admit
 Admitted.
 
 End Boolean_ber_decode.
